Prove dfs_complete.
This is quite a monstrous proof. At this point it starts making more
sense to rely on something like math-comp to deal with graphs. Their
proofs seem more compact, but I do not know how they work. The main
difficulty of my DFS algorithm is that the visited nodes are
propagated, such that each node is really only visited once.

I kept the soundess proof short at the cost of being a bit weaker;
it does not show that the resulting path avoids already visited nodes,
only that the returned path is a valid one.

dfs.v
@@ -1,6 +1,6 @@
 (* A depth-first search algorithm. *)
 
-Require Import Utf8 Wf_nat List.
+Require Import Utf8 PeanoNat List.
 From larith Require Import tactics notations utilities.
 Import ListNotations.
 
@@ -10,21 +10,42 @@ Variable X : Type.
 Variable R : X -> X -> Prop.
 
 Inductive RTC : list X -> Prop :=
-  | rtc_refl x : RTC [x]
-  | rtc_cons x y l : RTC (y :: l) -> R x y -> RTC (x :: y :: l).
+  | RTC_nil : RTC []
+  | RTC_refl x : RTC [x]
+  | RTC_cons x y l : RTC (y :: l) -> R x y -> RTC (x :: y :: l).
 
-Theorem RTC_trans l1 x1 x2 l2 :
-  RTC (l1 ++ [x1]) -> RTC (x2 :: l2) -> R x1 x2 ->
-  RTC (l1 ++ x1 :: x2 :: l2).
+Theorem RTC_trans l1 l2 d :
+  RTC l1 -> RTC (last l1 d :: l2) -> RTC (l1 ++ l2).
 Proof.
-induction l1; simpl; intros. apply rtc_cons; easy.
-destruct l1; simpl in *; inv H; repeat apply rtc_cons.
-4: apply IHl1. all: easy.
+induction l1; simpl; intros. inv H0.
+destruct l1; subst; simpl in *. easy.
+inv H; apply RTC_cons. apply IHl1; easy. easy.
+Qed.
+
+Theorem RTC_app_inv l1 l2 :
+  RTC (l1 ++ l2) -> RTC l1 /\ RTC l2.
+Proof.
+induction l1; simpl; intros.
+split; [apply RTC_nil|easy]. inv H.
+- apply eq_sym, app_eq_nil in H2 as [H1 H2]; subst.
+  split; [apply RTC_refl|apply RTC_nil].
+- rewrite H1 in H2; apply IHl1 in H2. split; [|easy].
+  destruct l1; [apply RTC_refl|inv H1; apply RTC_cons; easy].
 Qed.
 
 End Reflexive_transitive_closure.
 
 Arguments RTC {_}.
+
+Section Path_search.
+
+Notation Inr x := (∃r, x = inr r).
+
+Lemma Inr_inr {X Y} y :
+  Inr (@inr X Y y).
+Proof.
+exists y; reflexivity.
+Qed.
 
 Section Stateful_search.
 
@@ -36,26 +57,37 @@ Fixpoint search s l : state + (X × solution) :=
   | []      => inl s
   | x :: l' =>
     match check s x with
-    | inl s' => search s' l'
-    | inr y  => inr (x, y)
+    | inl t => search t l'
+    | inr y => inr (x, y)
     end
   end.
 
-Section Soundness.
-
-Variable P : X -> solution -> Prop.
-Hypothesis check_sound : ∀s x sol, check s x = inr sol -> P x sol.
-
-Theorem search_sound s l x sol :
-  search s l = inr (x, sol) -> In x l /\ P x sol.
+Theorem search_app s l1 l2 :
+  search s (l1 ++ l2) =
+  match search s l1 with
+  | inl t => search t l2
+  | _     => search s l1
+  end.
 Proof.
-revert s; induction l; simpl; intros. easy.
-destruct (check s a) eqn:Ha.
-apply IHl in H; split; [now right|apply H].
-inv H; split; [now left|eapply check_sound, Ha].
+revert s; induction l1; simpl; intros. easy.
+destruct (check s a); [apply IHl1|easy].
 Qed.
 
-End Soundness.
+Corollary search_app_Inr s l1 l2 :
+  Inr (search s l1) -> Inr (search s (l1 ++ l2)).
+Proof.
+intros [y Hy]; rewrite search_app, Hy.
+exists y; reflexivity.
+Qed.
+
+Theorem search_inr_inv s l x y :
+  search s l = inr (x, y) -> In x l /\ ∃t, check t x = inr y.
+Proof.
+revert s; induction l; simpl; intros. easy.
+destruct (check s a) as [t|y'] eqn:Ha.
+apply IHl in H; split; [now right|apply H].
+inv H; split; [now left|exists s; apply Ha].
+Qed.
 
 End Stateful_search.
 
@@ -68,61 +100,190 @@ Variable adj : node -> list node.
 Variable accept : node -> bool.
 Hypothesis dec : ∀v w : node, {v = w} + {v ≠ w}.
 
+Notation diff x y := (subtract dec x y).
+Notation next v := (remove dec v (adj v)).
+Notation Path := (RTC (λ v w, In w (next v))).
+Notation Notin l := (λ x, ¬In x l).
+
 Fixpoint dfs depth visited v : list node + list node :=
   match depth with
   | 0   => inl visited
   | S n =>
     if in_dec dec v visited then inl visited
     else if accept v then inr []
-    else match search (dfs n) (v :: visited) (adj v)
+    else match search (dfs n) (v :: visited) (next v)
     with
     | inl vis     => inl vis
     | inr (w, tr) => inr (w :: tr)
     end
   end.
 
-Notation diff x y := (subtract dec x y).
-Notation Inr x := (∃r, x = inr r).
-Notation Path := (RTC (λ v w, In w (adj v))).
+Definition DFS_path visited path :=
+  Path path /\ Forall (Notin visited) path.
+Definition DFS_solution visited v path :=
+  DFS_path visited (v :: path) /\ accept (last path v) = true.
 
-Definition DFS_solution_weak v tr :=
-  Path (v :: tr) /\ accept (last tr v) = true.
-Definition DFS_solution visited v tr :=
-  DFS_solution_weak v tr /\ Forall (λ v, ¬In v visited) (v :: tr).
-
-Theorem dfs_sound_weak depth visited v tr :
-  dfs depth visited v = inr tr -> DFS_solution_weak v tr.
+Lemma Forall_Notin_nil {X} (l : list X) :
+  Forall (Notin []) l.
 Proof.
-revert visited v tr; induction depth; simpl; intros. easy.
-destruct (in_dec dec v visited). easy.
-destruct (accept v) eqn:C. inv H; split; [apply rtc_refl|apply C].
-destruct (search _) eqn:Hs. easy. destruct p as [v' tr']; inv H.
-apply search_sound with (P:=DFS_solution_weak) in Hs as [H []].
-split. apply rtc_cons; easy. rewrite last_cons; apply H1.
-apply IHdepth.
+apply Forall_forall; easy.
+Qed.
+
+(* Solutions given by dfs are correct. *)
+Theorem dfs_sound_weak n visited v path :
+  dfs n visited v = inr path -> DFS_solution [] v path.
+Proof.
+revert visited v path; induction n; simpl; intros. easy.
+destruct (in_dec dec v visited). easy. destruct (accept v) eqn:C.
+inv H; repeat split; [apply RTC_refl|apply Forall_Notin_nil|apply C].
+destruct (search _) as [|[w path']] eqn:Hs; [easy|inv H].
+apply search_inr_inv in Hs as [Hw [t Ht]]; apply IHn in Ht as [[]].
+repeat split. now apply RTC_cons. apply Forall_Notin_nil. now rewrite last_cons.
+Qed.
+
+(* Visited nodes are remembered. *)
+Lemma dfs_inl_incl n vis_a v vis_z z :
+  dfs n vis_a v = inl vis_z -> In z vis_a -> In z vis_z.
+Proof.
+revert vis_a v vis_z; induction n; simpl; intros. inv H.
+destruct (in_dec _); [inv H|].
+destruct (accept v); [easy|].
+destruct (search _) as [vis_z'|[]] eqn:Hs; [inv H|easy].
+remember (v :: vis_a) as vis_b.
+assert(In z vis_b) by (subst; apply in_cons, H0).
+clear H0 Heqvis_b; revert H Hs; revert vis_b.
+induction (next v) as [|w ws]; simpl; intros.
+inv Hs. destruct (dfs _) as [vis_c|] eqn:Hw; [|easy].
+(* The inclusion relation is preserved over the induction. *)
+destruct (in_dec dec z vis_c); [|exfalso].
+apply IHws with (vis_b:=vis_c); easy.
+apply IHn in Hw; easy.
+Qed.
+
+(* Each new visited node can be reached by a path. *)
+Lemma path_to_visited n vis_a v vis_z z :
+  dfs n vis_a v = inl vis_z -> ¬In z vis_a -> In z vis_z ->
+  ∃path, DFS_path vis_a (v :: path) /\ last path v = z.
+Proof.
+revert vis_a v vis_z; induction n; simpl; intros. inv H.
+destruct (in_dec _); [inv H|].
+destruct (accept v); [easy|].
+destruct (search _) as [vis_z'|[]] eqn:Hs; [inv H|easy].
+(* Discard the case z = v. *)
+destruct (dec z v). exists []; subst; repeat split.
+apply RTC_refl. apply Forall_cons; easy.
+(* Abstract over (v :: vis_a) and (next v). *)
+remember (v :: vis_a) as vis_b; remember (next v) as nextv.
+assert(¬In z vis_b) by (subst; apply not_in_cons; easy).
+assert(∀x, In x vis_a -> In x vis_b) by (intros; subst; apply in_cons, H2).
+assert(∀x, In x nextv -> In x (next v)) by (subst; easy).
+clear H0 n1 Heqvis_b Heqnextv; revert Hs H H2; revert vis_b.
+induction nextv as [|w ws]; simpl; intros. inv Hs.
+(* Destruct the recursive call, and check if it visits z. *)
+destruct (dfs _) as [vis_c|] eqn:Hw; [|easy].
+destruct (in_dec dec z vis_c).
+- (* If the recursive call visits z; use IHn. *)
+  apply IHn in Hw as [path []]; try easy.
+  exists (w :: path); split; [|rewrite last_cons; apply H4].
+  destruct H0; split. apply RTC_cons; [apply H0|apply H3, in_eq].
+  apply Forall_cons. easy. eapply Forall_impl. 2: apply H5.
+  intros u; eapply contra, H2.
+- (* If it doesn't; use IHnextv. *)
+  apply IHws with (vis_b:=vis_c); try easy.
+  intros; apply H3; apply in_cons, H0.
+  intros; eapply dfs_inl_incl. apply Hw. apply H2, H0.
+Qed.
+
+(* Two DFS paths can be appended. *)
+Lemma DFS_path_trans visited v path1 path2 :
+  DFS_path visited (v :: path1) ->
+  DFS_path visited (last path1 v :: path2) ->
+  DFS_path visited (v :: path1 ++ path2).
+Proof.
+intros [H1a H1b] [H2a H2b].
+rewrite app_comm_cons; split. eapply RTC_trans with (d:=v).
+apply H1a. rewrite last_cons; apply H2a.
+apply Forall_app; split; [apply H1b|inv H2b].
 Qed.
 
 Variable graph : list node.
 Hypothesis graph_spec : ∀v, In v graph.
 
-Theorem dfs_complete visited v tr :
-  DFS_solution visited v tr ->
-  Inr (dfs (length (diff graph visited)) visited v).
+Theorem dfs_complete vis_a n :
+  length (diff graph vis_a) <= n ->
+  ∀v path, DFS_solution vis_a v path -> Inr (dfs n vis_a v).
 Proof.
-remember (length (diff graph visited)) as n eqn:len;
-revert len; revert visited v tr.
-apply lt_wf_rect with (n:=n); clear n; intros; destruct n.
-- (* Contradition; v ∈ graph \ visited. *)
-  destruct H0 as [_ H0]; inv H0.
-  exfalso; apply in_nil with (a:=v).
-  apply eq_sym, length_zero_iff_nil in len; rewrite <-len.
-  apply subtract_spec; easy.
-- (* The search through (adj v) must yield a solution. *)
-  destruct H0; inv H1; simpl.
-  destruct (in_dec _) as [F|_]; [easy|].
-  destruct (accept v) eqn:Hv; [now exists []|].
-Admitted.
+revert vis_a; induction n; intros vis_a Hn; intros.
+(* I. Zero case. Contradition since v ∈ graph \ visited. *)
+destruct H as [[_ H]]; inv H.
+exfalso; apply in_nil with (a:=v).
+apply Le.le_n_0_eq, eq_sym, length_zero_iff_nil in Hn.
+rewrite <-Hn; apply subtract_spec; easy.
+(* II. Successor case. *)
+destruct H as [[]]; inv H0; simpl.
+destruct (in_dec _) as [F|_]; [easy|].
+destruct (accept v) eqn:Hv; [apply Inr_inr|].
+(* Get a sub-path without v. *)
+destruct split_at_last_instance with (x:=v)(l:=v::path)
+as [pre [path' []]]. apply dec. apply in_eq.
+rewrite <-last_cons with (d:=v) in H1; rewrite H0 in H, H1.
+apply RTC_app_inv in H as [_ H]; rewrite last_app in H1.
+assert(Forall (Notin vis_a) path'). {
+  destruct pre; inv H0. apply Forall_app in H5 as [_ H5]; inv H5. }
+clear H0 H5 path pre.
+(* The given path cannot be empty; obtain the next node. *)
+inv H3; [simpl in H1; rewrite H1 in Hv; easy|].
+inv H; rewrite last_cons in H1; apply in_remove in H9 as ?.
+rename x into w, l into path.
+(* Wrap hypotheses back together and clean up. *)
+assert(H' : DFS_solution (v :: vis_a) w path). {
+  repeat split; try easy. apply Forall_cons.
+  apply not_in_cons; easy. apply not_in_cons in H2.
+  apply Forall_forall; intros u Hu [F|F]; subst. easy.
+  eapply Forall_forall with (x:=u) in H5; easy. }
+assert(Hn' : length (diff graph (v :: vis_a)) <= n). {
+  simpl; eapply Lt.lt_n_Sm_le, Nat.lt_le_trans.
+  apply subtract_length_lt_cons_r; [apply graph_spec|apply H4]. apply Hn. }
+clear H H0 H1 H2 H4 H5 H7 Hv Hn.
+remember (v :: vis_a) as vis_b; clear Heqvis_b vis_a.
+(* Split (next v) into (next1 ++ w :: next2). *)
+apply split_list in H9 as [next1 [next2 H9]]; rewrite H9.
+cut(Inr (search (dfs n) vis_b (next1 ++ [w]))). intros Hr.
+apply search_app_Inr with (l2:=next2) in Hr as [[u path'] Hr].
+rewrite <-app_assoc in Hr; simpl in Hr; rewrite Hr; apply Inr_inr.
+clear H9 v; revert H' Hn'; revert vis_b.
+(* Do induction on the nodes that are checked before w. *)
+induction next1 as [|u]; simpl; intros.
+- (* At w the previous induction hypothesis guarantees a solution. *)
+  apply IHn in H' as [path' H']. rewrite H'; apply Inr_inr. easy.
+- (* Check if the search terminates before w. *)
+  destruct (dfs _) as [vis_c|] eqn:Hu; [|apply Inr_inr].
+  (* If not, then we can use IHnext1. *)
+  apply IHnext1; clear IHnext1 next1.
+  + (* Show that the path does not go through visited nodes. *)
+    destruct H' as [[]]; repeat split; try easy.
+    rewrite Forall_Exists_neg, Exists_exists; intros [e [H1e H2e]].
+    apply Forall_forall with (x:=e) in H0 as H3e; [|apply H1e].
+    (* If it does, then there exists a contradictory solution for v. *)
+    eapply path_to_visited in H2e as [to_e ?]; [|apply Hu|apply H3e].
+    destruct H2; subst. apply split_list in H1e as [path1 [path2 H1e]].
+    rewrite <-last_cons with (d:=w) in H1; rewrite H1e in H, H0, H1.
+    apply RTC_app_inv in H as [_ H]; apply Forall_app in H0 as [_ H0];
+    rewrite last_app in H1.
+    (* to_e ++ path2 is now a solution for u. *)
+    assert(DFS_solution vis_b u (to_e ++ path2)).
+    * split. apply DFS_path_trans; easy.
+      destruct path2. rewrite app_nil_r; apply H1.
+      rewrite last_app; rewrite last_cons in H1; apply H1.
+    * apply IHn in H3. rewrite Hu in H3; destruct H3; easy. easy.
+  + (* Show that n is big enough. *)
+    etransitivity; [|apply Hn'].
+    apply length_subtract_le_incl_r.
+    intros; eapply dfs_inl_incl; [apply Hu|apply H].
+Qed.
 
 End Depth_first_search.
+
+End Path_search.
 
 Arguments dfs {_}.
